Join_discrete no longer has an implicit argument

msl/examples/sep/corec_example.v
@@ -1,7 +1,7 @@
 Require Import msl.msl_direct.
 
 Definition heap : Type := fpm nat nat.
-Instance Join_heap: Join heap := Join_fpm (@Join_discrete _).
+Instance Join_heap: Join heap := Join_fpm (Join_discrete _).
 
 Instance Perm_heap: Perm_alg heap := Perm_fpm _ (Perm_discrete nat).
 
@@ -10,17 +10,17 @@ Definition mapsto  (x y: nat) : pred heap :=
 
 Inductive lis' : nat -> pred heap :=
 | lis_nil : forall p w, (!!(p=0) && emp)%pred w -> lis' p w
-| lis_cons: forall p w, (!!(p<>0) && Ex r:nat, mapsto p r * lis' r)%pred w -> lis' p w.
+| lis_cons: forall p w, (!!(p<>0) && EX r:nat, mapsto p r * lis' r)%pred w -> lis' p w.
 
 Lemma lis'_fold_unfold:
-    forall p, lis' p =  (!!(p=0) && emp || !!(p<>0) && Ex r:nat, mapsto p r * lis' r)%pred.
+    forall p, lis' p =  (!!(p=0) && emp || !!(p<>0) && EX r:nat, mapsto p r * lis' r)%pred.
 Proof.
 intros.
 apply pred_ext; intros w ?; (inv H; [left | right]; auto).
 Qed.
 
 Definition lisfun (Q: nat -> pred heap) (p: nat)  : pred heap:=
-  (!!(p=0) && emp || !!(p<>0) && Ex r:nat, mapsto p r * Q r)%pred.
+  (!!(p=0) && emp || !!(p<>0) && EX r:nat, mapsto p r * Q r)%pred.
 
 Lemma covariant_lisfun: covariant lisfun.
 Proof.
@@ -37,7 +37,7 @@ Qed.
 Definition lis : nat -> pred heap := corec lisfun.
 
 Lemma lis_fold_unfold:
-    forall p, lis p =  (!!(p=0) && emp || !!(p<>0) && Ex r:nat, mapsto p r * lis r)%pred.
+    forall p, lis p =  (!!(p=0) && emp || !!(p<>0) && EX r:nat, mapsto p r * lis r)%pred.
 Proof.
 intros.
 unfold lis at 1.
